repair second SimplifyCFG decision boundaries

lowering/defs/evalCompilerBytecodeSecondSimplifyCfgCollapseDecisionsScript.sml
@@ -6,19 +6,44 @@ open HolKernel Parse boolLib bossLib
 
 val () = computeLib.upd_compset finite_mapLib.add_finite_map_compset
 
+fun head_is c t = same_const (fst (strip_comb t)) c handle HOL_ERR _ => false
+fun has_head c t = head_is c t orelse can (find_term (head_is c)) t
 fun assert_closed label tm =
   if null (free_vars tm) then ()
   else raise Fail (label ^ " is not closed: " ^ term_to_string tm)
+fun assert_reduced label query_head th =
+  let
+    val (l, r) = dest_eq (concl th)
+  in
+    if aconv l r then raise Fail (label ^ " produced a reflexive equation")
+    else if has_head query_head r then
+      raise Fail (label ^ " left its query head on the RHS")
+    else assert_closed label (concl th)
+  end
 
+val operand_def =
+  evalCompilerBytecodeSecondSimplifyCfgResultTheory.second_simplify_cfg_operand_def
+val removed_def =
+  evalCompilerBytecodeSecondSimplifyCfgInitialRemoveTheory.second_simplify_cfg_removed_def
+val phi_fixed_def =
+  evalCompilerBytecodeSecondSimplifyCfgInitialPhiTheory.second_simplify_cfg_phi_fixed_def
 val second_literal_edge_ths =
-  map (REWRITE_RULE
-    [evalCompilerBytecodeSecondSimplifyCfgResultTheory.second_simplify_cfg_operand_def])
+  map (REWRITE_RULE [operand_def])
     [second_simplify_cfg_dispatch_edge, second_simplify_cfg_fallback_edge]
-val second_phi_fixed_blocks_th =
-  SIMP_RULE (srw_ss ()) second_literal_edge_ths
-    second_simplify_cfg_phi_fixed_blocks
+val second_removed_normal_th =
+  SIMP_RULE (srw_ss ()) second_literal_edge_ths removed_def
+val second_phi_fixed_normal_th =
+  SIMP_RULE (srw_ss ())
+    (second_removed_normal_th :: second_literal_edge_ths) phi_fixed_def
+val second_phi_fixed_tm = rhs (concl second_phi_fixed_normal_th)
+val _ = assert_closed "literal second PHI-fixed function" second_phi_fixed_tm
+val second_phi_fixed_blocks_projection_th =
+  computeLib.EVAL_CONV
+    (mk_comb (``\fn : ir_function. fn.fn_blocks``, second_phi_fixed_tm))
+val second_phi_fixed_blocks_tm =
+  rhs (concl second_phi_fixed_blocks_projection_th)
 val second_phi_fixed_blocks =
-  fst (listSyntax.dest_list (rhs (concl second_phi_fixed_blocks_th)))
+  fst (listSyntax.dest_list second_phi_fixed_blocks_tm)
 val _ =
   if length second_phi_fixed_blocks = 3 then ()
   else raise Fail "second PHI-fixed function changed fixture block count"
@@ -38,58 +63,84 @@ End
 Definition second_simplify_cfg_fallback_bb_def:
   second_simplify_cfg_fallback_bb = ^second_fallback_bb_tm
 End
+val second_phi_fixed_blocks_named_th =
+  CONV_RULE (DEPTH_CONV BETA_CONV)
+    (PURE_REWRITE_RULE
+      [GSYM second_simplify_cfg_entry_bb_def,
+       GSYM second_simplify_cfg_dispatch_bb_def,
+       GSYM second_simplify_cfg_fallback_bb_def]
+      (TRANS
+        (AP_TERM ``\fn : ir_function. fn.fn_blocks`` second_phi_fixed_normal_th)
+        second_phi_fixed_blocks_projection_th))
 
-val phi_fixed_def =
-  evalCompilerBytecodeSecondSimplifyCfgInitialPhiTheory.second_simplify_cfg_phi_fixed_def
-fun eval_phi_fixed tm =
-  SIMP_CONV (srw_ss ()) [phi_fixed_def] tm
+fun literal_query c args = list_mk_comb (c, args)
+fun eval_literal label query_head tm =
+  let
+    val th = computeLib.EVAL_CONV tm
+    val _ = assert_reduced label query_head th
+  in
+    th
+  end
 
-val second_entry_lookup_th = eval_phi_fixed
-  ``lookup_block "__entry" second_simplify_cfg_phi_fixed.fn_blocks``
-val second_dispatch_lookup_th = eval_phi_fixed
-  ``lookup_block "@dispatch_1" second_simplify_cfg_phi_fixed.fn_blocks``
-val second_fallback_lookup_th = eval_phi_fixed
-  ``lookup_block "@fallback_0" second_simplify_cfg_phi_fixed.fn_blocks``
-val second_entry_succs_th = computeLib.EVAL_CONV
-  ``bb_succs second_simplify_cfg_entry_bb``
-val second_dispatch_succs_th = computeLib.EVAL_CONV
-  ``bb_succs second_simplify_cfg_dispatch_bb``
-val second_fallback_succs_th = computeLib.EVAL_CONV
-  ``bb_succs second_simplify_cfg_fallback_bb``
-val _ =
-  if aconv (rhs (concl second_entry_succs_th))
-       ``["@fallback_0"; "@dispatch_1"]``
-  then () else raise Fail "second entry successor order changed"
-val _ =
-  if aconv (rhs (concl second_dispatch_succs_th)) ``["@fallback_0"]``
-  then () else raise Fail "second dispatch successor order changed"
-val _ =
-  if aconv (rhs (concl second_fallback_succs_th)) ``[] : string list``
-  then () else raise Fail "second fallback successor order changed"
+val second_entry_lookup_raw = eval_literal "entry lookup" ``lookup_block``
+  (literal_query ``lookup_block`` [``"__entry"``, second_phi_fixed_blocks_tm])
+val second_dispatch_lookup_raw = eval_literal "dispatch lookup" ``lookup_block``
+  (literal_query ``lookup_block`` [``"@dispatch_1"``, second_phi_fixed_blocks_tm])
+val second_fallback_lookup_raw = eval_literal "fallback lookup" ``lookup_block``
+  (literal_query ``lookup_block`` [``"@fallback_0"``, second_phi_fixed_blocks_tm])
+val second_entry_succs_raw = eval_literal "entry successors" ``bb_succs``
+  (mk_comb (``bb_succs``, second_entry_bb_tm))
+val second_dispatch_succs_raw = eval_literal "dispatch successors" ``bb_succs``
+  (mk_comb (``bb_succs``, second_dispatch_bb_tm))
+val second_fallback_succs_raw = eval_literal "fallback successors" ``bb_succs``
+  (mk_comb (``bb_succs``, second_fallback_bb_tm))
+val second_fallback_preds_raw = eval_literal "fallback predecessor count" ``num_preds``
+  (literal_query ``num_preds`` [second_phi_fixed_tm, ``"@fallback_0"``])
+val second_entry_try_bypass_raw = eval_literal "entry try_bypass" ``try_bypass``
+  (literal_query ``try_bypass``
+    [second_phi_fixed_tm, ``[] : (string # string) list``, second_entry_bb_tm,
+     ``["@fallback_0"; "@dispatch_1"]``])
+val second_dispatch_merge_fallback_raw = eval_literal "dispatch/fallback merge" ``can_merge_blocks``
+  (literal_query ``can_merge_blocks``
+    [second_phi_fixed_tm, second_dispatch_bb_tm, second_fallback_bb_tm])
 
-val second_fallback_preds_th = eval_phi_fixed
-  ``num_preds second_simplify_cfg_phi_fixed "@fallback_0"``
-val second_entry_try_bypass_th = eval_phi_fixed
-  ``try_bypass second_simplify_cfg_phi_fixed []
-      second_simplify_cfg_entry_bb ["@fallback_0"; "@dispatch_1"]``
-val second_dispatch_merge_fallback_th = eval_phi_fixed
-  ``can_merge_blocks second_simplify_cfg_phi_fixed
-      second_simplify_cfg_dispatch_bb second_simplify_cfg_fallback_bb``
+val naming_rewrites =
+  [GSYM second_phi_fixed_normal_th,
+   GSYM second_simplify_cfg_entry_bb_def,
+   GSYM second_simplify_cfg_dispatch_bb_def,
+   GSYM second_simplify_cfg_fallback_bb_def,
+   GSYM second_phi_fixed_blocks_named_th]
+fun name_decision th = PURE_REWRITE_RULE naming_rewrites th
+val second_entry_lookup_th = name_decision second_entry_lookup_raw
+val second_dispatch_lookup_th = name_decision second_dispatch_lookup_raw
+val second_fallback_lookup_th = name_decision second_fallback_lookup_raw
+val second_entry_succs_th = name_decision second_entry_succs_raw
+val second_dispatch_succs_th = name_decision second_dispatch_succs_raw
+val second_fallback_succs_th = name_decision second_fallback_succs_raw
+val second_fallback_preds_th = name_decision second_fallback_preds_raw
+val second_entry_try_bypass_th = name_decision second_entry_try_bypass_raw
+val second_dispatch_merge_fallback_th =
+  name_decision second_dispatch_merge_fallback_raw
 
-val second_closed_decision_ths =
-  [second_entry_lookup_th, second_dispatch_lookup_th,
-   second_fallback_lookup_th, second_entry_succs_th,
-   second_dispatch_succs_th, second_fallback_succs_th,
-   second_fallback_preds_th, second_entry_try_bypass_th,
-   second_dispatch_merge_fallback_th]
-val _ =
-  map (assert_closed "second SimplifyCFG collapse decision" o concl)
-    second_closed_decision_ths
-
-Theorem exact_second_simplify_cfg_closed_decisions:
-  ^(concl (LIST_CONJ second_closed_decision_ths))
+Theorem exact_second_entry_lookup:
+  lookup_block "__entry" second_simplify_cfg_phi_fixed.fn_blocks =
+    SOME second_simplify_cfg_entry_bb
 Proof
-  ACCEPT_TAC (LIST_CONJ second_closed_decision_ths)
+  ACCEPT_TAC second_entry_lookup_th
+QED
+
+Theorem exact_second_dispatch_lookup:
+  lookup_block "@dispatch_1" second_simplify_cfg_phi_fixed.fn_blocks =
+    SOME second_simplify_cfg_dispatch_bb
+Proof
+  ACCEPT_TAC second_dispatch_lookup_th
+QED
+
+Theorem exact_second_fallback_lookup:
+  lookup_block "@fallback_0" second_simplify_cfg_phi_fixed.fn_blocks =
+    SOME second_simplify_cfg_fallback_bb
+Proof
+  ACCEPT_TAC second_fallback_lookup_th
 QED
 
 Theorem exact_second_entry_succs:
@@ -97,6 +148,41 @@ Theorem exact_second_entry_succs:
     ["@fallback_0"; "@dispatch_1"]
 Proof
   ACCEPT_TAC second_entry_succs_th
+QED
+
+Theorem exact_second_dispatch_succs:
+  bb_succs second_simplify_cfg_dispatch_bb = ["@fallback_0"]
+Proof
+  ACCEPT_TAC second_dispatch_succs_th
+QED
+
+Theorem exact_second_fallback_succs:
+  bb_succs second_simplify_cfg_fallback_bb = []
+Proof
+  ACCEPT_TAC second_fallback_succs_th
+QED
+
+Theorem exact_second_fallback_preds:
+  num_preds second_simplify_cfg_phi_fixed "@fallback_0" = 2
+Proof
+  ACCEPT_TAC second_fallback_preds_th
+QED
+
+Theorem exact_second_entry_try_bypass:
+  try_bypass second_simplify_cfg_phi_fixed [] second_simplify_cfg_entry_bb
+    ["@fallback_0"; "@dispatch_1"] =
+  (second_simplify_cfg_phi_fixed, [], F)
+Proof
+  rewrite_tac [second_entry_try_bypass_th] >>
+  pure_rewrite_tac [second_phi_fixed_normal_th, operand_def] >>
+  simp[venomInstTheory.ir_function_component_equality]
+QED
+
+Theorem exact_second_dispatch_merge_fallback:
+  can_merge_blocks second_simplify_cfg_phi_fixed
+    second_simplify_cfg_dispatch_bb second_simplify_cfg_fallback_bb = F
+Proof
+  ACCEPT_TAC second_dispatch_merge_fallback_th
 QED
 
 val _ = export_theory()
